spectec/test-rocq/theories/subtyping.v
@@ -1,0 +1,447 @@
+From Stdlib Require Import List Bool Nat Arith.
+Import ListNotations.
+From WasmSpectec Require Import wasm helper_lemmas helper_tactics.
+From mathcomp Require Import ssreflect ssrfun ssrnat ssrbool seq eqtype.
+
+Notation "tf1 :-> tf2" :=
+(mk_functype (mk_list _ tf1) (mk_list _ tf2)) (at level 40).
+
+Notation "t1 <t? t2" := (Valtype_sub t1 t2) (at level 30).
+Definition Resulttype_subtype ts1 ts2 := Resulttype_sub (mk_list _ ts1) (mk_list _ ts2).
+Notation "ts1 <ts? ts2" := (Resulttype_subtype ts1 ts2) (at level 60).
+
+Definition Ftype_sub tf1 tf2 : Prop :=
+  match tf1, tf2 with
+  | ts11 :-> ts12,
+    ts21 :-> ts22 =>
+        (ts21 <ts? ts11) /\
+        (ts12 <ts? ts22)
+  end.
+
+Definition instrtype_sub tf tf' : Prop :=
+  match tf, tf' with
+  | ts1 :-> ts2,
+    ts1' :-> ts2' =>
+        exists ts_sub ts ts1_sub ts2_sup,
+        ts1' = ts_sub ++ ts1 /\
+        ts2' = ts ++ ts2_sup /\
+        (ts_sub <ts? ts) /\
+        (ts1_sub <ts? ts1) /\
+        (ts2 <ts? ts2_sup)
+  end.
+
+Notation "tf1 <tf? tf2" := (Ftype_sub tf1 tf2) (at level 60).
+Notation "tf1 <ti: tf2" := (instrtype_sub tf1 tf2) (at level 60).
+
+Lemma size_length : forall {A : Type} (xs : seq A),
+  size xs = length xs.
+Proof. auto. Qed.
+
+Lemma valtype_sub_refl : forall t, t <t? t.
+Proof.
+  move => t.
+  apply refl.
+Qed.
+
+Lemma valtype_sub_trans: forall t1 t2 t3,
+    t1 <t? t2 ->
+    t2 <t? t3 ->
+    t1 <t? t3.
+Proof.
+  move => t1 t2 t3 H12 H23.
+  destruct t1, t2, t3; eauto; try apply refl; try apply bot;
+  try inversion H23; try inversion H12.
+Qed.
+
+Lemma resulttype_sub_refl : forall ts, ts <ts? ts.
+Proof.
+  intros ts.
+  constructor; auto.
+  induction ts as [|t ts IH]; simpl; auto.
+  constructor; auto.
+  apply valtype_sub_refl.
+Qed.
+
+Lemma resulttype_sub_size_eq: forall ts1 ts2,
+    ts1 <ts? ts2 ->
+    size ts1 = size ts2.
+Proof.
+  move => ts1 ts2 H.
+  inversion H; subst.
+  auto.
+Qed.
+
+Lemma resulttype_sub_trans: forall ts1 ts2 ts3,
+    ts1 <ts? ts2 ->
+    ts2 <ts? ts3 ->
+    ts1 <ts? ts3.
+Proof.
+  move => ts1 ts2 ts3 H12 H23.
+  inversion H12; inversion H23; subst.
+  constructor.
+  - by rewrite H1.
+  - move : ts2 ts3 H12 H23 H1 H2 H5 H6.
+    induction ts1 as [| t1 ts1 IH];
+    destruct ts2 as [| t2 ts2];
+    destruct ts3 as [| t3 ts3]; try discriminate;
+    try constructor.
+    + inversion H2; inversion H6; subst.
+      eapply valtype_sub_trans; eauto.
+    + rewrite !length_cons in H1;
+      inversion H1.
+      rewrite !length_cons in H5;
+      inversion H5.
+      inversion H2; inversion H6; subst.
+      apply (IH ts2 ts3);
+      auto; constructor; auto.
+Qed.
+
+Lemma resulttype_sub_app_trans: forall ts_sub ts ts1 ts2,
+    ts_sub <ts? ts ->
+    (ts ++ ts1) <ts? (ts2) ->
+    (ts_sub ++ ts1) <ts? (ts2).
+Proof.
+  move => ts_sub ts ts1 ts2 H1 H2.
+  constructor.
+  - inversion H1; inversion H2; subst.
+    rewrite -H7.
+    rewrite -!size_length.
+    rewrite !size_cat.
+    rewrite !size_length.
+    by rewrite H3.
+  - move: ts ts1 ts2 H1 H2. 
+    induction ts_sub as [| t_sub ts_sub IH];
+    destruct ts as [| t ts];
+    destruct ts2 as [| t2 ts2];
+    move=> H1 H2;
+    try (inversion H1; inversion H2; discriminate);
+    try (by inversion H2).
+    rewrite cat_cons.
+    rewrite cat_cons in H2.
+    inversion H1; inversion H2; subst; clear H1 H2.
+    inversion H4; inversion H8; subst; clear H4 H8.
+    constructor.
+    { eapply valtype_sub_trans; eauto. } 
+    eapply IH.
+    + inversion H3.
+      econstructor ; eauto.
+    * inversion H7.
+      econstructor; auto.
+Qed.
+
+Lemma all2_cat' : forall A (f : A -> A -> bool) l1 l2 l3 l4,
+  size l1 = size l2 ->
+  all2 f (l1 ++ l3) (l2 ++ l4) ->
+  all2 f l1 l2 /\ all2 f l3 l4.
+Proof.
+  induction l1 as [| a1 l1 IH];
+  destruct l2 as [| a2 l2]; move => l3 l4 HSize H; split;
+  simpl in H; try discriminate HSize; auto;
+  move/andP: H => [H1 H2];
+  inversion HSize;
+  eapply IH in H0 as [H3 H4].
+  - simpl. apply/andP; split; auto.
+  eauto. eauto. eauto.
+Qed.
+
+Lemma all2_cat : forall A (f : A -> A -> bool) l1 l2 l3 l4,
+  all2 f l1 l2 -> all2 f l3 l4 ->
+  all2 f (l1 ++ l3) (l2 ++ l4).
+Proof.
+  induction l1 as [| a1 l1 IH];
+  destruct l2 as [| a2 l2];
+  destruct l3 as [| a3 l3];
+  destruct l4 as [| a4 l4];
+  auto.
+  - move => H12 _.
+    by repeat rewrite cats0.
+  - move => H1 H2.
+    rewrite cat_cons.
+    simpl.
+    apply/andP; split.
+    + simpl in H1. by move/andP: H1 => [H1 _].
+    + apply IH.
+      * simpl in H1. by move/andP: H1 => [_ H1].
+      * auto.
+Qed.
+
+Lemma resulttype_sub_app: forall ts1_sub ts2_sub ts1 ts2,
+  (ts1_sub <ts? ts1) ->
+  (ts2_sub <ts? ts2) ->
+  (ts1_sub ++ ts2_sub) <ts? (ts1 ++ ts2).
+Proof.
+  induction ts1_sub as [| t1_sub ts1_sub IH];
+  move=> ts2_sub ts1 ts2 H1 H2.
+  - inversion H1; subst.
+    simpl in H3; symmetry in H3.
+    rewrite length_zero_iff_nil in H3.
+    subst.
+    by rewrite !cat0s.
+  - destruct ts1 as [| t1 ts1].
+    { inversion H1; discriminate. }
+    rewrite !cat_cons.
+    inversion H1; subst; clear H1.
+    constructor.
+    + simpl; f_equal.
+      inversion H2; subst.
+      simpl in H3; inversion H3.
+      rewrite -!size_length.
+      rewrite !size_cat.
+      rewrite !size_length.
+      rewrite H1; rewrite H0; reflexivity.
+    + inversion H4; subst; clear H4.
+      constructor; auto.
+      simpl in H3; inversion H3; subst; clear H3.
+      apply Forall2_app.
+      { by apply H7. }
+      by inversion H2.
+Qed.
+
+Lemma Forall2_app': forall {A B : Type} (R : A -> B -> Prop)
+  (l1 l2 : seq A) (l1' l2' : seq B),
+  length l1 = length l1' ->
+  Forall2 R (l1 ++ l2) (l1' ++ l2') ->
+  Forall2 R l1 l1' /\ Forall2 R l2 l2'.
+Proof.
+  induction l1 as [| x l1 IH];
+  destruct l1' as [| x' l1']; auto; try discriminate.
+  move=> l2' Hsize H1.
+  rewrite !cat_cons in H1.
+  inversion Hsize; clear Hsize.
+  eapply IH in H0 as [Hl1 Hl2].
+  split.
+  - constructor. by inversion H1.
+  - by apply Hl1.
+  - eauto.
+  - by inversion H1.
+Qed.
+
+Lemma resulttype_sub_app': forall ts1_sub ts2_sub ts1 ts2,
+  length ts1_sub = length ts1 ->
+  (ts1_sub ++ ts2_sub) <ts? (ts1 ++ ts2) ->
+  (ts1_sub <ts? ts1) /\
+  (ts2_sub <ts? ts2).
+Proof.
+  move => ts1_sub ts2_sub ts1 ts2 Hsize Happ.
+  inversion Happ; subst.
+  split; constructor; auto; 
+  eapply (Forall2_app' Valtype_sub) in H2 as [HF1 HF2]; eauto.
+  rewrite -!size_length in Hsize H1.
+  rewrite -!size_length.
+  rewrite !size_cat in H1.
+  rewrite Hsize in H1.
+  by rewrite Nat.add_cancel_l in H1.
+Qed.
+
+Lemma Forall2_take : forall {A B: Type} (R : A -> B -> Prop) l1 l2 n,
+  Forall2 R l1 l2 ->
+  Forall2 R (take n l1) (take n l2).
+Proof.
+  induction l1 as [| e1 l1 IH]; destruct l2 as [| e2 l2];
+  move => n H; try inversion H; subst;
+  destruct n as [|n]; simpl; auto.
+Qed.
+
+Lemma Forall2_drop : forall {A B: Type} (R : A -> B -> Prop) l1 l2 n,
+  Forall2 R l1 l2 ->
+  Forall2 R (drop n l1) (drop n l2).
+Proof.
+  induction l1 as [| e1 l1 IH]; destruct l2 as [| e2 l2];
+  move => n H; try inversion H; subst;
+  destruct n as [|n]; simpl; auto.
+Qed.
+
+Lemma resulttype_sub_split: forall ts1 ts2 n,
+    (ts1 <ts? ts2) ->
+    ((take n ts1) <ts? (take n ts2)) /\
+    ((drop n ts1) <ts? (drop n ts2)).
+Proof.
+  move => ts1 ts2 n Hsub.
+  have Hsize: size ts1 = size ts2 by apply resulttype_sub_size_eq.
+  inversion Hsub; subst.
+  split.
+  - constructor.
+    + eapply Forall2_length.
+      eapply Forall2_take.
+      eauto.
+    + by eapply Forall2_take.
+  - constructor.
+    + eapply Forall2_length.
+      eapply Forall2_drop.
+      eauto.
+    + by eapply Forall2_drop.
+Qed.
+
+Lemma lt_irrefl: forall x, x < x = false.
+Proof.
+  move => x.
+  induction x as [| n IH]; simpl; auto.
+Qed.
+
+Lemma drop_size_cat : forall A (x y : seq A),
+  drop (size x) (x ++ y) = y.
+Proof.
+  move => A x y.
+  rewrite drop_cat.
+  rewrite ltnn.
+  rewrite subnn.
+  by rewrite drop0.
+Qed.
+
+Lemma take_size_cat : forall A (x y : seq A),
+  take (size x) (x ++ y) = x.
+Proof.
+  move => A x y.
+  rewrite take_cat.
+  rewrite ltnn.
+  rewrite subnn.
+  rewrite take0.
+  apply cats0.
+Qed.
+
+Lemma resulttype_sub_split_sup: forall ts ts1 ts2,
+    ts <ts? (ts1 ++ ts2) ->
+    ((take (size ts1) ts) <ts? ts1) /\
+    ((drop (size ts1) ts) <ts? ts2).
+Proof.
+  move => ts ts1 ts2 Hsub.
+  assert (ts1 = take (size ts1) (ts1 ++ ts2)) as Htake.
+  { symmetry. apply take_size_cat.  }
+  assert (ts2 = drop (size ts1) (ts1 ++ ts2)) as Hdrop.
+  { symmetry. apply drop_size_cat. }
+  eapply resulttype_sub_split in Hsub.
+  rewrite <- Htake in Hsub.
+  rewrite <- Hdrop in Hsub.
+  auto.
+Qed.
+
+Lemma ftype_sub_refl : forall tf, tf <tf? tf.
+Proof.
+  move => [[ts1] [ts2]].
+  unfold Ftype_sub.
+  split; apply resulttype_sub_refl.
+Qed.
+
+Lemma ftype_sub_trans: forall tf1 tf2 tf3,
+    tf1 <tf? tf2 ->
+    tf2 <tf? tf3 ->
+    tf1 <tf? tf3.
+Proof.
+  move => [[ts11] [ts12]] [[ts21] [ts22]] [[ts31] [ts32]] H12 H23.
+  unfold Ftype_sub in *; simpl in *.
+  destruct H12 as [H12_1 H12_2];
+  destruct H23 as [H23_1 H23_2].
+  split; eapply resulttype_sub_trans; eauto.
+Qed.
+
+Lemma instrtype_sub_refl: forall tf, tf <ti: tf.
+Proof.
+  move => [[ts1] [ts2]].
+  unfold instrtype_sub.
+  exists [], [], ts1, ts2.
+  assert (forall ts, Forall2 (Valtype_sub) ts ts).
+  move => ts.
+  induction ts as [| t ts IH]; auto.
+  constructor.
+  apply valtype_sub_refl.
+  auto.
+  repeat split; auto.
+Qed.
+
+Lemma instrtype_sub_trans: forall tf1 tf2 tf3,
+    tf1 <ti: tf2 ->
+    tf2 <ti: tf3 ->
+    tf1 <ti: tf3.
+Proof.
+  move => [[ts11] [ts12]] [[ts21] [ts22]] [[ts31] [ts32]] H12 H23.
+  unfold instrtype_sub in *.
+  destruct H12 as [tsH12_sub [tsH12 [ts11_sub [ts12_sup [
+    H12_1 [H12_2 [H12_3 [H12_4 H12_5]]]]]]]];
+  destruct H23 as [tsH23_sub [tsH23 [ts21_sub [ts22_sup [
+    H23_1 [H23_2 [H23_3 [H23_4 H23_5]]]]]]]];
+  subst.
+
+  eexists (tsH23_sub ++ tsH12_sub),
+    (tsH23 ++ take (List.length tsH12) ts22_sup), 
+    (ts11_sub), ((drop (List.length tsH12) ts22_sup)).
+
+  assert (size tsH12 <= size ts22_sup) as HSize.
+  { apply resulttype_sub_size_eq in H23_5.
+    rewrite <- H23_5.
+    apply size_prefix.
+    apply prefix_prefix.
+  }
+  rewrite <- (cat_take_drop (length tsH12) ts22_sup) in H23_5.
+  assert (size tsH12 = size (take (length tsH12) ts22_sup)).
+  {
+    by apply size_takel in HSize.
+  }
+  apply resulttype_sub_app' in H23_5 as [H23_51 H23_52].
+
+  split.
+  { rewrite <- app_assoc.
+    reflexivity. }
+  split.
+  { rewrite <- app_assoc.
+    by erewrite cat_take_drop. }
+  split.
+  { apply resulttype_sub_app; auto.
+    eapply resulttype_sub_trans; eauto.
+  }
+  split; auto.
+  { eapply resulttype_sub_trans; eauto. }
+  auto.
+Qed.
+  
+
+#[global]
+Instance valuetype_sub_preorder: RelationClasses.PreOrder Valtype_sub.
+Proof.
+  constructor.
+  - move => x. by apply valtype_sub_refl.
+  - move => x y z Hxy Hyz. eapply valtype_sub_trans; eauto.
+Qed.
+
+#[global]
+Instance resulttype_sub_preorder: RelationClasses.PreOrder Resulttype_sub.
+Proof.
+  constructor.
+  - move => x. destruct x. apply resulttype_sub_refl.
+  - move => x y z Hxy Hyz. destruct x, y, z. eapply resulttype_sub_trans; eauto.
+Qed.
+
+#[global]
+Instance ftype_sub_preorder: RelationClasses.PreOrder Ftype_sub.
+Proof.
+  constructor.
+  - move => x. by apply ftype_sub_refl.
+  - move => x y z Hxy Hyz. eapply ftype_sub_trans; eauto.
+Qed.
+
+#[global]
+Instance instrtype_sub_preorder: RelationClasses.PreOrder instrtype_sub.
+Proof.
+  constructor.
+  - move => x. by apply instrtype_sub_refl.
+  - move => x y z Hxy Hyz. eapply instrtype_sub_trans; eauto.
+Qed.
+
+Lemma resulttype_sub_empty : forall ts,
+  (ts <ts? []) ->
+  (ts = []).
+Proof.
+  move => ts H.
+  inversion H; subst.
+  simpl in H2.
+  by eapply length_zero_iff_nil.
+Qed.
+
+Lemma resulttype_empty_sub : forall ts,
+  ([] <ts? ts) ->
+  (ts = []).
+Proof.
+  move => ts H.
+  inversion H; subst.
+  simpl in H2.
+  by eapply length_zero_iff_nil.
+Qed.
